got size_diff proven using the recursive definition of its running time

size/size_log_sq.v
@@ -1,34 +1,24 @@
 Require Import Braun.common.braun Braun.common.log Braun.common.util Braun.common.log_sq.
-Require Import Braun.tmonad.monad.
-Require Import Coq.Program.Wf Arith.Even Arith.Div2 Arith.
+Require Import Braun.tmonad.monad Braun.common.big_oh.
+Require Import Coq.Program.Wf Arith.Even Arith.Div2 Arith Init.Wf.
+
+Include WfExtensionality.
+
+Program Fixpoint diff_time m {measure m} :=
+  match m with
+    | 0 => 4
+    | S m' =>
+      if (even_odd_dec m)
+      then 13 + diff_time (div2 (m' - 1))
+      else 11 + diff_time (div2 m')
+  end.
 
 Definition diff_result (A:Set) (b : @bin_tree A) m n c :=
-   (Braun b m     -> (n = 0 /\ c = fl_log m)) 
+   (Braun b m     -> (n = 0 /\ c = diff_time m))
    /\
-   (Braun b (m+1) -> (n = 1 /\ c = fl_log m + 1)).
+   (Braun b (m+1) -> (n = 1 /\ c = diff_time m)).
 
-(* this is generated from the rkt code, but 
-   tweaked to have the same constants as the
-   hand-written version *)
-Program Fixpoint diff {A:Set} (b:@bin_tree A) (m:nat) {measure m}
-: {! res !:! nat !<! c !>!
-     diff_result A b m res c !} :=
-  match b, m with
-    | bt_mt, _ => 
-      += 0; 
-      <== 0
-    | bt_node x _ _, 0 => 
-      += 1; 
-      <== 1
-    | bt_node x s t, S m' => 
-      if (even_odd_dec m)
-      then (o <- diff t (div2 (m' - 1));
-            += 1; 
-            <== o)
-      else (o <- diff s (div2 m');
-            += 1; 
-            <== o)
-  end.
+Load "diff_gen.v".
 
 Next Obligation.
   unfold diff_result in *.
@@ -40,7 +30,18 @@ Qed.
 Next Obligation.
   unfold diff_result in *.
   simpl.
+  unfold_sub diff_time (diff_time 0).
   split; intros B; invclr B; omega.
+Qed.
+
+Lemma diff_time_nz_even : 
+  forall m', even (S m') -> diff_time (S m') = 13+diff_time (div2 (m'-1)).
+  intros m' EV.
+  unfold_sub diff_time (diff_time (S m')).
+  fold diff_time.
+  dispatch_if x x'; auto.
+  assert False; intuition.
+  apply (not_even_and_odd (S m')); auto.
 Qed.
 
 Next Obligation.
@@ -50,6 +51,8 @@ Next Obligation.
   destruct BTxn as [BT1 BT2].
 
   unfold diff_result in *.
+  rewrite diff_time_nz_even; auto.
+
   apply even_2n in E. destruct E as [mm EQ].
   unfold double in EQ.
   split; intros B; invclr B;
@@ -64,9 +67,9 @@ Next Obligation.
   apply BT1 in Bt.
   destruct Bt as [Bt_o Bt_xn].
   subst. split; auto.
-  apply braun_invariant_implies_fl_log_property.
-  auto.
-  symmetry. apply div2_double.
+  omega. unfold mult. 
+  replace (t_size + (t_size + 0)) with (t_size+t_size); try omega.
+  symmetry. apply double_div2.
 
   replace s_size with t_size in *; try omega.
   clear BP s_size.
@@ -80,15 +83,27 @@ Next Obligation.
   replace (t_size + 1) with (S t_size) in *; try omega.
   apply BT2 in Bt.
   destruct Bt as [Bt_o Bt_xn].
-  subst. split; auto.
-  rewrite <- fl_log_even.
-  replace (t_size + 1 + (t_size + 1)) with (S (t_size + S t_size)); omega.
+  subst. split; auto. 
+  omega.
+Qed.
+
+Lemma diff_time_nz_odd : 
+  forall m', odd (S m') -> diff_time (S m') = 11+diff_time (div2 m').
+  intros m' EV.
+  unfold_sub diff_time (diff_time (S m')).
+  fold diff_time.
+  dispatch_if x x'; auto.
+  assert False; intuition.
+  apply (not_even_and_odd (S m')); auto.
 Qed.
 
 Next Obligation.
   clear am H2 diff.
   rename H1 into BT.
   rename H into O.
+
+  unfold diff_result in *.
+  rewrite diff_time_nz_odd; auto.
 
   destruct BT as [BT1 BT2].
   apply odd_S2n in O. destruct O as [mm EQ].
@@ -106,38 +121,29 @@ Next Obligation.
   apply BT1 in Bs.
   destruct Bs as [Bt_o Bt_xn]. subst.
   split; auto.
-  rewrite <- fl_log_odd.
-  replace (t_size + t_size + 1) with (S (2 * t_size)); omega.
+  omega.
 
   replace s_size with (t_size + 1) in *; try omega.
   replace mm with t_size in *; try omega.
   apply BT2 in Bs.
   destruct Bs as [Bt_o Bt_xn]. subst.
   split; auto.
-  rewrite <- fl_log_odd.
-  replace (t_size + t_size + 1) with (S (2 * t_size)); omega.
+  omega.
 Qed.
+
+
+Program Fixpoint size_time n {measure n} :=
+  match n with
+    | 0 => 3
+    | S n' => 
+      13 + diff_time (div2 n') + size_time (div2 n')
+  end.
 
 Definition size_result (A:Set) (b : @bin_tree A) n c :=
   forall m,
-    (Braun b m -> (n = m /\ c = sum_of_logs n)).
+    (Braun b m -> (n = m /\ c = size_time n)).
 
-(* this is generated from the rkt code, but 
-   tweaked to have the same constants as the
-   hand-written version *)
-Program Fixpoint size {A:Set} (b:@bin_tree A)
-: {! res !:! nat !<! c !>!
-     size_result A b res c !} :=
-  match b with
-    | bt_mt => 
-      += 0; 
-      <== 0
-    | bt_node _ s t => 
-      m <- size t;
-      zo <- diff s m;
-      += 1; 
-      <== (1 + (2 * m) + zo)
-  end.
+Load "size_log_sq_gen.v".
 
 Next Obligation.
 Proof.
@@ -157,6 +163,8 @@ Proof.
   destruct DIFF_RES as [SIZE_SAME SIZE_DIFF].
 
   unfold size_result in *.
+  unfold_sub size_time (size_time (S (m + (m + 0) + zo))).
+(*  replace (m + (m + 0) + zo) *)
 
   intros m0 BTb.
 
@@ -171,20 +179,19 @@ Proof.
 
   assert (s_size = t_size \/ s_size = t_size + 1) as TWOCASES;[omega|].
   destruct TWOCASES as [EQ|EQ]; subst.
-
   apply SIZE_SAME in BRAUNS. destruct BRAUNS as [EQo EQxn]. subst.
+  replace (t_size + (t_size + 0) + 0) with (t_size + t_size); [|omega].
+  rewrite double_div2.
   split; try omega.
-  replace (S (t_size + (t_size + 0) + 0)) with (t_size+t_size+1);[|omega].
-  rewrite <- sum_of_logs_odd.
-  rewrite fl_log_odd.
-  omega.
 
   apply SIZE_DIFF in BRAUNS. destruct BRAUNS as [EQo EQxn]. subst.
+  replace (t_size + (t_size + 0) + 1) with (S (t_size + t_size)); [|omega].
+  rewrite div2_with_odd_argument.
   split; try omega.
-  replace (S (t_size + (t_size + 0) + 1)) with (t_size + 1 + t_size + 1);[|omega].
-  rewrite <- sum_of_logs_even.
-  rewrite <- cl_log_even.
-  replace (t_size + 1) with (S t_size);[|omega].
-  rewrite <- fl_log_cl_log_relationship.
-  omega.
 Qed.
+
+Theorem size_logsq : big_oh size_time (fun n => cl_log n * cl_log n).
+Proof.
+  admit.
+Qed.
+
